src/proof/controllers/statefulset/pod_predicates.v
@@ -1,37 +1,4 @@
-From New.proof Require Export wp_helpers.
-From New.proof.string Require Export prefix_suffix.
-From New.proof.kubernetes_types Require Export prelude.
-From New.proof.controllers Require Export common.
-From New.proof.controllers.statefulset Require Import pvc_predicates.
-
-Definition statefulset_replicas (sts : StatefulSetV.t) : nat :=
-  match sts.(StatefulSetV.Spec').(StatefulSetSpecV.Replicas') with
-  | Some replicas => sint.nat replicas
-  | None => 1%nat
-  end.
-
-Definition desired_ordinals (sts : StatefulSetV.t) : list nat :=
-  seq 0 (statefulset_replicas sts).
-
-Definition desired_pod_name (set_name : go_string) (ordinal : nat) : go_string :=
-  set_name ++ "-"%go ++ decimal_string ordinal.
-
-Definition desired_pod_key sts ordinal : KKey.t := {|
-  KKey.Kind' := PodV.kind;
-  KKey.Namespace' := sts.(StatefulSetV.ObjectMeta').(ObjectMetaV.Namespace');
-  KKey.Name' := desired_pod_name
-    sts.(StatefulSetV.ObjectMeta').(ObjectMetaV.Name') ordinal;
-|}.
-
-Definition desired_pod_keys (sts : StatefulSetV.t) : list KKey.t :=
-  desired_pod_key sts <$> desired_ordinals sts.
-
-Definition pod_key_is_desired (sts : StatefulSetV.t) (key : KKey.t) : Prop :=
-  key ∈ desired_pod_keys sts.
-
-#[global] Instance pod_key_is_desired_decision sts key :
-    Decision (pod_key_is_desired sts key).
-Proof. unfold pod_key_is_desired. apply _. Defined.
+From New.proof.controllers.statefulset Require Export top_level.
 
 Definition pod_has_member_name (set_name pod_name : go_string) : Prop :=
   ∃ ordinal, pod_name = desired_pod_name set_name ordinal.
@@ -77,45 +44,6 @@ Proof.
   rewrite elem_of_cons. by left.
 Qed.
 
-Definition member_name_prefix (set_name : go_string) : go_string :=
-  set_name ++ "-"%go.
-
-Definition parse_member_name (set_name pod_name : go_string) : option nat :=
-  match New.proof.string.prefix_suffix.strip_prefix (member_name_prefix set_name)
-      pod_name with
-  | Some suffix => parse_canonical_decimal_string suffix
-  | None => None
-  end.
-
-Lemma parse_member_name_sound set_name pod_name ordinal :
-  parse_member_name set_name pod_name = Some ordinal →
-  pod_name = desired_pod_name set_name ordinal.
-Proof.
-  unfold parse_member_name.
-  destruct (New.proof.string.prefix_suffix.strip_prefix (member_name_prefix set_name)
-    pod_name) as [suffix|] eqn:Hstrip; [|done].
-  intros Hparse.
-  apply parse_canonical_decimal_string_sound in Hparse.
-  apply New.proof.string.prefix_suffix.strip_prefix_correct in Hstrip.
-  unfold desired_pod_name, member_name_prefix in *.
-  rewrite Hstrip.
-  rewrite -Hparse.
-  by rewrite List.app_assoc.
-Qed.
-
-Lemma parse_member_name_complete set_name pod_name ordinal :
-  pod_name = desired_pod_name set_name ordinal →
-  parse_member_name set_name pod_name = Some ordinal.
-Proof.
-  intros Hname.
-  unfold parse_member_name.
-  rewrite Hname.
-  unfold desired_pod_name, member_name_prefix.
-  rewrite List.app_assoc.
-  rewrite New.proof.string.prefix_suffix.strip_prefix_complete.
-  apply parse_canonical_decimal_string_decimal_string.
-Qed.
-
 #[global] Instance pod_has_member_name_decision set_name pod_name :
   Decision (pod_has_member_name set_name pod_name).
 Proof.
@@ -125,37 +53,6 @@ Proof.
     apply parse_member_name_complete in Hname.
     congruence.
 Defined.
-
-Definition pod_has_int32_member_name (set_name pod_name : go_string) : Prop :=
-  ∃ ordinal : nat,
-    (ordinal <= go_int32_max_nat)%nat ∧
-    pod_name = desired_pod_name set_name ordinal.
-
-#[global] Instance pod_has_int32_member_name_decision set_name pod_name :
-    Decision (pod_has_int32_member_name set_name pod_name).
-Proof.
-  unfold pod_has_int32_member_name.
-  destruct (parse_member_name set_name pod_name) as [ordinal|] eqn:Hparse.
-  - destruct (decide (ordinal <= go_int32_max_nat)%nat) as [Hbound|Hoverflow].
-    + left. exists ordinal. split; [done|].
-      by apply parse_member_name_sound.
-    + right. intros (ordinal' & Hbound & Hname).
-      apply parse_member_name_complete in Hname.
-      rewrite Hparse in Hname.
-      simplify_eq/=.
-      done.
-  - right. intros (ordinal & _ & Hname).
-    apply parse_member_name_complete in Hname.
-    congruence.
-Defined.
-
-(* These are precisely the Pods that pass [filterPodsForStatefulSet] and cause
-   [reconcileReplicas] to return when it observes their deletion timestamp. *)
-Definition pending_pod sts (pod : PodV.t) : Prop :=
-  ¬ is_pod_alive pod ∧
-  pod_has_int32_member_name
-    sts.(StatefulSetV.ObjectMeta').(ObjectMetaV.Name')
-    pod.(PodV.ObjectMeta').(ObjectMetaV.Name').
 
 Lemma pod_has_member_key_iff sts pod :
   pod_has_member_key sts pod ↔
@@ -190,16 +87,6 @@ Proof.
   - right. intros Hmember_key.
     apply Hnot_member. by apply pod_has_member_key_iff.
 Defined.
-
-Definition pod_ordinal_suffix (pod_name : go_string) : option go_string :=
-  match list_find (λ b, b = byte_dash) (reverse pod_name) with
-  | Some (idx, _) => Some (reverse (take idx (reverse pod_name)))
-  | None => None
-  end.
-
-Definition parse_pod_ordinal (pod_name : go_string) : option nat :=
-  suffix ← pod_ordinal_suffix pod_name;
-  parse_decimal_string suffix.
 
 Lemma pod_name_length_le_go_int_max_of_valid_name name :
   valid_name PodV.kind name →
@@ -266,132 +153,6 @@ Proof.
   rewrite New.proof.string.prefix_suffix.strip_prefix_complete in Hparse.
   simpl in Hparse. done.
 Qed.
-
-Definition pod_identity_matches (sts : StatefulSetV.t) (pod : PodV.t) : Prop :=
-  match parse_member_name
-      sts.(StatefulSetV.ObjectMeta').(ObjectMetaV.Name')
-      pod.(PodV.ObjectMeta').(ObjectMetaV.Name'),
-    pod.(PodV.ObjectMeta').(ObjectMetaV.Labels') with
-  | Some ordinal, Some labels =>
-      (ordinal <= go_int32_max_nat)%nat ∧
-      pod.(PodV.ObjectMeta').(ObjectMetaV.Namespace') =
-        sts.(StatefulSetV.ObjectMeta').(ObjectMetaV.Namespace') ∧
-      labels !! statefulset_pod_name_label =
-        Some pod.(PodV.ObjectMeta').(ObjectMetaV.Name') ∧
-      labels !! pod_index_label = Some (decimal_string ordinal)
-  | _, _ => False
-  end.
-
-#[global] Instance pod_identity_matches_decision sts pod :
-    Decision (pod_identity_matches sts pod).
-Proof.
-  unfold pod_identity_matches.
-  destruct parse_member_name,
-    (pod.(PodV.ObjectMeta').(ObjectMetaV.Labels')); apply _.
-Defined.
-
-(* Go map insertion overwrites an earlier volume with the same name, so the
-   left fold preserves the last volume from the Pod's volume slice. *)
-Definition pod_volumes_map_insert
-    (volumes : gmap go_string VolumeV.t) (volume : VolumeV.t) :
-    gmap go_string VolumeV.t :=
-  <[volume.(VolumeV.Name') := volume]> volumes.
-
-Definition pod_volumes_map_of_list (volumes : list VolumeV.t) :
-    gmap go_string VolumeV.t :=
-  fold_left pod_volumes_map_insert volumes ∅.
-
-Definition pod_volume_claim_matches
-    (volumes : gmap go_string VolumeV.t) (set_name : go_string)
-    (ordinal : nat) (claim_template_name : go_string) : Prop :=
-  match volumes !! claim_template_name with
-  | Some volume =>
-      match volume.(VolumeV.VolumeSource').(
-        VolumeSourceV.PersistentVolumeClaim') with
-      | Some pvc =>
-          pvc.(v1.PersistentVolumeClaimVolumeSource.ClaimName') =
-            desired_pvc_name set_name claim_template_name ordinal
-      | None => False
-      end
-  | None => False
-  end.
-
-#[global] Instance pod_volume_claim_matches_decision volumes set_name ordinal
-    claim_template_name :
-    Decision (pod_volume_claim_matches volumes set_name ordinal
-      claim_template_name).
-Proof.
-  unfold pod_volume_claim_matches.
-  destruct (volumes !! claim_template_name) as [volume|]; [|apply _].
-  destruct volume.(VolumeV.VolumeSource').(
-    VolumeSourceV.PersistentVolumeClaim'); apply _.
-Defined.
-
-Definition pod_storage_matches (set : StatefulSetV.t) (pod : PodV.t) : Prop :=
-  match parse_pod_ordinal
-      pod.(PodV.ObjectMeta').(ObjectMetaV.Name') with
-  | Some ordinal =>
-      (ordinal <= go_int32_max_nat)%nat ∧
-      Forall
-        (pod_volume_claim_matches
-          (pod_volumes_map_of_list pod.(PodV.Spec').(PodSpecV.Volumes'))
-          set.(StatefulSetV.ObjectMeta').(ObjectMetaV.Name') ordinal)
-        (pvc_claim_template_names set)
-  | None => False
-  end.
-
-#[global] Instance pod_storage_matches_decision set pod :
-    Decision (pod_storage_matches set pod).
-Proof.
-  unfold pod_storage_matches.
-  destruct (parse_pod_ordinal
-    pod.(PodV.ObjectMeta').(ObjectMetaV.Name')); apply _.
-Defined.
-
-Definition without_statefulset_fields (_ : PodSpecV.t) : PodSpecV.t := {|
-  PodSpecV.Volumes' := [];
-  PodSpecV.Hostname' := ""%go;
-  PodSpecV.Subdomain' := ""%go;
-|}.
-
-(* [podSpecMatches] treats Hostname, Subdomain, and the StatefulSet PVC
-   volumes as immutable creation-time state. The remaining PodSpec fields must
-   still agree with the Pod template after those generated fields are erased. *)
-Definition pod_immutable_matches (sts : StatefulSetV.t) (pod : PodV.t) : Prop :=
-  pod.(PodV.Spec').(PodSpecV.Hostname') =
-    pod.(PodV.ObjectMeta').(ObjectMetaV.Name') ∧
-  pod.(PodV.Spec').(PodSpecV.Subdomain') =
-    sts.(StatefulSetV.Spec').(StatefulSetSpecV.ServiceName') ∧
-  pod_storage_matches sts pod ∧
-  without_statefulset_fields pod.(PodV.Spec') =
-    without_statefulset_fields
-      sts.(StatefulSetV.Spec').(StatefulSetSpecV.Template').(PodTemplateSpecV.Spec').
-
-#[global] Instance pod_immutable_matches_decision sts pod :
-    Decision (pod_immutable_matches sts pod).
-Proof.
-  unfold pod_immutable_matches, without_statefulset_fields.
-  destruct (decide
-    (pod.(PodV.Spec').(PodSpecV.Hostname') =
-      pod.(PodV.ObjectMeta').(ObjectMetaV.Name'))) as [Hhostname|Hhostname].
-  2: { right. intros (H & _). contradiction. }
-  destruct (decide
-    (pod.(PodV.Spec').(PodSpecV.Subdomain') =
-      sts.(StatefulSetV.Spec').(StatefulSetSpecV.ServiceName')))
-    as [Hsubdomain|Hsubdomain].
-  2: { right. intros (_ & H & _). contradiction. }
-  destruct (decide (pod_storage_matches sts pod))
-    as [Hstorage|Hstorage].
-  2: { right. intros (_ & _ & H & _). contradiction. }
-  left. split_and!; try done.
-Defined.
-
-Definition pod_match (sts : StatefulSetV.t) (pod : PodV.t) : Prop :=
-  pod_identity_matches sts pod ∧
-  pod_immutable_matches sts pod.
-
-#[global] Instance pod_match_decision sts pod : Decision (pod_match sts pod).
-Proof. unfold pod_match. apply _. Defined.
 
 Definition pod_is_condemned (set : StatefulSetV.t) (pod : PodV.t) : Prop :=
   ∃ ordinal,
