src/proof/controllers/statefulset/ordinal.v
@@ -1,3 +1,4 @@
+From New.proof.controllers.statefulset Require Import top_level.
 From New.proof.controllers Require Export common.
 From New.proof.controllers.statefulset Require Import pod_predicates.
 From New.proof.controllers.statefulset Require Export statefulset_init.
