src/proof/controllers/statefulset/outdated.v
@@ -1,3 +1,4 @@
+From New.proof.controllers.statefulset Require Import top_level.
 From New.proof.controllers.statefulset Require Export pod_predicates.
 From New.proof.controllers.statefulset Require Export ordinal.
 
