src/proof/controllers/statefulset/reconcile_stability.v
@@ -1,3 +1,4 @@
+From New.proof.controllers.statefulset Require Import top_level.
 From New.proof.controllers.statefulset Require Export reconcile_progress.
 From New.proof.controllers.statefulset Require Import create_pvc update_pod
   release condemned outdated.
