src/proof/controllers/statefulset/top_level.v
@@ -1,0 +1,577 @@
+From New.proof Require Export wp_helpers.
+From New.proof.string Require Export prefix_suffix.
+From New.proof.kubernetes_types Require Export prelude.
+From New.proof.controllers Require Export common.
+From New.proof.k8s_io.api.apps Require Export v1_init.
+From New.proof.k8s_io.api.core Require Export v1_init.
+From New.proof.k8s_io.apimachinery.pkg.api Require Export errors_init.
+From New.proof.k8s_io.apimachinery.pkg.apis.meta Require Export v1_init.
+From New.proof.k8s_io.kubernetes.pkg Require Export controller_init.
+From New.proof.kubernetes_model Require Export apimodel_init.
+From New.proof Require Export reflect_init strconv_init strings.
+From New.proof.controllers Require Export common_init.
+Require Export New.generatedproof.controllers.statefulset.
+From New.proof Require Import proof_prelude.
+
+Section init.
+Context `{hG: heapGS Σ} `{!ffi_semantics _ _}.
+Context {sem : go.Semantics} {package_sem : statefulset.Assumptions}.
+Collection W := sem + package_sem.
+
+#[global] Instance : IsPkgInit (iProp Σ) statefulset :=
+  define_is_pkg_init True%I.
+#[global] Instance : GetIsPkgInitWf (iProp Σ) statefulset :=
+  build_get_is_pkg_init_wf.
+End init.
+
+(* Pure desired-state definitions used by all three top-level specifications.
+   This file deliberately imports no other file from the statefulset proof
+   directory, so clients can depend on the specifications without importing
+   their proofs. *)
+
+Definition pvc_claim_template_names (sts : StatefulSetV.t) : list go_string :=
+  (λ claim_template,
+    claim_template.(PersistentVolumeClaimV.ObjectMeta').(ObjectMetaV.Name'))
+  <$> sts.(StatefulSetV.Spec').(StatefulSetSpecV.VolumeClaimTemplates').
+
+Definition desired_pvc_name set_name claim_template_name ordinal : go_string :=
+  claim_template_name ++ "-"%go ++ set_name ++ "-"%go ++ decimal_string ordinal.
+
+Definition desired_pvc_key sts claim_template_name ordinal : KKey.t := {|
+  KKey.Kind' := PersistentVolumeClaimV.kind;
+  KKey.Namespace' := sts.(StatefulSetV.ObjectMeta').(ObjectMetaV.Namespace');
+  KKey.Name' := desired_pvc_name
+    sts.(StatefulSetV.ObjectMeta').(ObjectMetaV.Name') claim_template_name ordinal;
+|}.
+
+Definition desired_pvc_key_candidates sts : list KKey.t :=
+  concat (
+    (λ ordinal,
+      (λ claim_template_name, desired_pvc_key sts claim_template_name ordinal)
+      <$> pvc_claim_template_names sts)
+    <$> seq 0
+      (match sts.(StatefulSetV.Spec').(StatefulSetSpecV.Replicas') with
+       | Some replicas => sint.nat replicas
+       | None => 1%nat
+       end)
+  ).
+
+Definition desired_pvc_keys sts : list KKey.t :=
+  elements (list_to_set (C:=gset KKey.t) (desired_pvc_key_candidates sts)).
+
+Definition new_persistent_volume_claim_labels
+    (set : StatefulSetV.t) (claim_template : PersistentVolumeClaimV.t) :
+    gmap go_string go_string :=
+  let claim_labels :=
+    default ∅
+      claim_template.(PersistentVolumeClaimV.ObjectMeta').(ObjectMetaV.Labels') in
+  let selector_labels :=
+    match set.(StatefulSetV.Spec').(StatefulSetSpecV.Selector') with
+    | Some selector =>
+        default ∅ selector.(LabelSelectorV.MatchLabels')
+    | None => ∅
+    end in
+  selector_labels ∪ claim_labels.
+
+Definition new_persistent_volume_claim
+    (set : StatefulSetV.t) (claim_template : PersistentVolumeClaimV.t)
+    (ordinal : nat) : PersistentVolumeClaimV.t :=
+  let object_meta :=
+    claim_template.(PersistentVolumeClaimV.ObjectMeta')
+      <| ObjectMetaV.Name' :=
+          desired_pvc_name
+            set.(StatefulSetV.ObjectMeta').(ObjectMetaV.Name')
+            claim_template.(PersistentVolumeClaimV.ObjectMeta').(ObjectMetaV.Name')
+            ordinal |>
+      <| ObjectMetaV.Namespace' :=
+          set.(StatefulSetV.ObjectMeta').(ObjectMetaV.Namespace') |>
+      <| ObjectMetaV.OwnerReferences' := None |>
+      <| ObjectMetaV.Labels' :=
+          Some (new_persistent_volume_claim_labels set claim_template) |> in
+  claim_template <| PersistentVolumeClaimV.ObjectMeta' := object_meta |>.
+
+Definition statefulset_replicas (sts : StatefulSetV.t) : nat :=
+  match sts.(StatefulSetV.Spec').(StatefulSetSpecV.Replicas') with
+  | Some replicas => sint.nat replicas
+  | None => 1%nat
+  end.
+
+Definition desired_ordinals (sts : StatefulSetV.t) : list nat :=
+  seq 0 (statefulset_replicas sts).
+
+Definition desired_pod_name (set_name : go_string) (ordinal : nat) : go_string :=
+  set_name ++ "-"%go ++ decimal_string ordinal.
+
+Definition desired_pod_key sts ordinal : KKey.t := {|
+  KKey.Kind' := PodV.kind;
+  KKey.Namespace' := sts.(StatefulSetV.ObjectMeta').(ObjectMetaV.Namespace');
+  KKey.Name' := desired_pod_name
+    sts.(StatefulSetV.ObjectMeta').(ObjectMetaV.Name') ordinal;
+|}.
+
+Definition desired_pod_keys (sts : StatefulSetV.t) : list KKey.t :=
+  desired_pod_key sts <$> desired_ordinals sts.
+
+Definition pod_key_is_desired (sts : StatefulSetV.t) (key : KKey.t) : Prop :=
+  key ∈ desired_pod_keys sts.
+
+#[global] Instance pod_key_is_desired_decision sts key :
+    Decision (pod_key_is_desired sts key).
+Proof. unfold pod_key_is_desired. apply _. Defined.
+
+Definition member_name_prefix (set_name : go_string) : go_string :=
+  set_name ++ "-"%go.
+
+Definition parse_member_name (set_name pod_name : go_string) : option nat :=
+  match New.proof.string.prefix_suffix.strip_prefix (member_name_prefix set_name)
+      pod_name with
+  | Some suffix => parse_canonical_decimal_string suffix
+  | None => None
+  end.
+
+Lemma parse_member_name_sound set_name pod_name ordinal :
+  parse_member_name set_name pod_name = Some ordinal →
+  pod_name = desired_pod_name set_name ordinal.
+Proof.
+  unfold parse_member_name.
+  destruct (New.proof.string.prefix_suffix.strip_prefix
+    (member_name_prefix set_name) pod_name) as [suffix|] eqn:Hstrip; [|done].
+  intros Hparse.
+  apply parse_canonical_decimal_string_sound in Hparse.
+  apply New.proof.string.prefix_suffix.strip_prefix_correct in Hstrip.
+  unfold desired_pod_name, member_name_prefix in *.
+  rewrite Hstrip -Hparse.
+  by rewrite List.app_assoc.
+Qed.
+
+Lemma parse_member_name_complete set_name pod_name ordinal :
+  pod_name = desired_pod_name set_name ordinal →
+  parse_member_name set_name pod_name = Some ordinal.
+Proof.
+  intros Hname.
+  unfold parse_member_name.
+  rewrite Hname.
+  unfold desired_pod_name, member_name_prefix.
+  rewrite List.app_assoc.
+  rewrite New.proof.string.prefix_suffix.strip_prefix_complete.
+  apply parse_canonical_decimal_string_decimal_string.
+Qed.
+
+Definition pod_has_int32_member_name (set_name pod_name : go_string) : Prop :=
+  ∃ ordinal : nat,
+    (ordinal <= go_int32_max_nat)%nat ∧
+    pod_name = desired_pod_name set_name ordinal.
+
+#[global] Instance pod_has_int32_member_name_decision set_name pod_name :
+    Decision (pod_has_int32_member_name set_name pod_name).
+Proof.
+  unfold pod_has_int32_member_name.
+  destruct (parse_member_name set_name pod_name) as [ordinal|] eqn:Hparse.
+  - destruct (decide (ordinal <= go_int32_max_nat)%nat) as
+      [Hbound|Hoverflow].
+    + left. exists ordinal. split; [done|].
+      by apply parse_member_name_sound.
+    + right. intros (ordinal' & Hbound & Hname).
+      apply parse_member_name_complete in Hname.
+      rewrite Hparse in Hname. simplify_eq/=. done.
+  - right. intros (ordinal & _ & Hname).
+    apply parse_member_name_complete in Hname. congruence.
+Defined.
+
+Definition pending_pod sts (pod : PodV.t) : Prop :=
+  ¬ is_pod_alive pod ∧
+  pod_has_int32_member_name
+    sts.(StatefulSetV.ObjectMeta').(ObjectMetaV.Name')
+    pod.(PodV.ObjectMeta').(ObjectMetaV.Name').
+
+#[global] Instance pending_pod_decision sts pod :
+    Decision (pending_pod sts pod).
+Proof. unfold pending_pod, is_pod_alive. apply _. Defined.
+
+Definition pod_ordinal_suffix (pod_name : go_string) : option go_string :=
+  match list_find (λ b, b = byte_dash) (reverse pod_name) with
+  | Some (idx, _) => Some (reverse (take idx (reverse pod_name)))
+  | None => None
+  end.
+
+Definition parse_pod_ordinal (pod_name : go_string) : option nat :=
+  suffix ← pod_ordinal_suffix pod_name;
+  parse_decimal_string suffix.
+
+Definition pod_identity_matches (sts : StatefulSetV.t) (pod : PodV.t) : Prop :=
+  match parse_member_name
+      sts.(StatefulSetV.ObjectMeta').(ObjectMetaV.Name')
+      pod.(PodV.ObjectMeta').(ObjectMetaV.Name'),
+    pod.(PodV.ObjectMeta').(ObjectMetaV.Labels') with
+  | Some ordinal, Some labels =>
+      (ordinal <= go_int32_max_nat)%nat ∧
+      pod.(PodV.ObjectMeta').(ObjectMetaV.Namespace') =
+        sts.(StatefulSetV.ObjectMeta').(ObjectMetaV.Namespace') ∧
+      labels !! statefulset_pod_name_label =
+        Some pod.(PodV.ObjectMeta').(ObjectMetaV.Name') ∧
+      labels !! pod_index_label = Some (decimal_string ordinal)
+  | _, _ => False
+  end.
+
+#[global] Instance pod_identity_matches_decision sts pod :
+    Decision (pod_identity_matches sts pod).
+Proof.
+  unfold pod_identity_matches.
+  destruct parse_member_name,
+    (pod.(PodV.ObjectMeta').(ObjectMetaV.Labels')); apply _.
+Defined.
+
+Definition pod_volumes_map_insert
+    (volumes : gmap go_string VolumeV.t) (volume : VolumeV.t) :
+    gmap go_string VolumeV.t :=
+  <[volume.(VolumeV.Name') := volume]> volumes.
+
+Definition pod_volumes_map_of_list (volumes : list VolumeV.t) :
+    gmap go_string VolumeV.t :=
+  fold_left pod_volumes_map_insert volumes ∅.
+
+Definition pod_volume_claim_matches
+    (volumes : gmap go_string VolumeV.t) (set_name : go_string)
+    (ordinal : nat) (claim_template_name : go_string) : Prop :=
+  match volumes !! claim_template_name with
+  | Some volume =>
+      match volume.(VolumeV.VolumeSource').(
+        VolumeSourceV.PersistentVolumeClaim') with
+      | Some pvc =>
+          pvc.(v1.PersistentVolumeClaimVolumeSource.ClaimName') =
+            desired_pvc_name set_name claim_template_name ordinal
+      | None => False
+      end
+  | None => False
+  end.
+
+#[global] Instance pod_volume_claim_matches_decision volumes set_name ordinal
+    claim_template_name :
+    Decision (pod_volume_claim_matches volumes set_name ordinal
+      claim_template_name).
+Proof.
+  unfold pod_volume_claim_matches.
+  destruct (volumes !! claim_template_name) as [volume|]; [|apply _].
+  destruct volume.(VolumeV.VolumeSource').(
+    VolumeSourceV.PersistentVolumeClaim'); apply _.
+Defined.
+
+Definition pod_storage_matches (set : StatefulSetV.t) (pod : PodV.t) : Prop :=
+  match parse_pod_ordinal pod.(PodV.ObjectMeta').(ObjectMetaV.Name') with
+  | Some ordinal =>
+      (ordinal <= go_int32_max_nat)%nat ∧
+      Forall
+        (pod_volume_claim_matches
+          (pod_volumes_map_of_list pod.(PodV.Spec').(PodSpecV.Volumes'))
+          set.(StatefulSetV.ObjectMeta').(ObjectMetaV.Name') ordinal)
+        (pvc_claim_template_names set)
+  | None => False
+  end.
+
+#[global] Instance pod_storage_matches_decision set pod :
+    Decision (pod_storage_matches set pod).
+Proof.
+  unfold pod_storage_matches.
+  destruct (parse_pod_ordinal
+    pod.(PodV.ObjectMeta').(ObjectMetaV.Name')); apply _.
+Defined.
+
+Definition without_statefulset_fields (_ : PodSpecV.t) : PodSpecV.t := {|
+  PodSpecV.Volumes' := [];
+  PodSpecV.Hostname' := ""%go;
+  PodSpecV.Subdomain' := ""%go;
+|}.
+
+Definition pod_immutable_matches (sts : StatefulSetV.t) (pod : PodV.t) : Prop :=
+  pod.(PodV.Spec').(PodSpecV.Hostname') =
+    pod.(PodV.ObjectMeta').(ObjectMetaV.Name') ∧
+  pod.(PodV.Spec').(PodSpecV.Subdomain') =
+    sts.(StatefulSetV.Spec').(StatefulSetSpecV.ServiceName') ∧
+  pod_storage_matches sts pod ∧
+  without_statefulset_fields pod.(PodV.Spec') =
+    without_statefulset_fields
+      sts.(StatefulSetV.Spec').(StatefulSetSpecV.Template').(
+        PodTemplateSpecV.Spec').
+
+#[global] Instance pod_immutable_matches_decision sts pod :
+    Decision (pod_immutable_matches sts pod).
+Proof.
+  unfold pod_immutable_matches, without_statefulset_fields.
+  destruct (decide
+    (pod.(PodV.Spec').(PodSpecV.Hostname') =
+      pod.(PodV.ObjectMeta').(ObjectMetaV.Name'))) as [Hhostname|Hhostname].
+  2: { right. intros (H & _). contradiction. }
+  destruct (decide
+    (pod.(PodV.Spec').(PodSpecV.Subdomain') =
+      sts.(StatefulSetV.Spec').(StatefulSetSpecV.ServiceName')))
+    as [Hsubdomain|Hsubdomain].
+  2: { right. intros (_ & H & _). contradiction. }
+  destruct (decide (pod_storage_matches sts pod)) as [Hstorage|Hstorage].
+  2: { right. intros (_ & _ & H & _). contradiction. }
+  left. split_and!; try done.
+Defined.
+
+Definition pod_match (sts : StatefulSetV.t) (pod : PodV.t) : Prop :=
+  pod_identity_matches sts pod ∧ pod_immutable_matches sts pod.
+
+#[global] Instance pod_match_decision sts pod : Decision (pod_match sts pod).
+Proof. unfold pod_match. apply _. Defined.
+
+Definition pod_has_int32_member_key
+    (sts : StatefulSetV.t) (pod : PodV.t) : Prop :=
+  pod.(PodV.ObjectMeta').(ObjectMetaV.Namespace') =
+    sts.(StatefulSetV.ObjectMeta').(ObjectMetaV.Namespace') ∧
+  pod_has_int32_member_name
+    sts.(StatefulSetV.ObjectMeta').(ObjectMetaV.Name')
+    pod.(PodV.ObjectMeta').(ObjectMetaV.Name').
+
+#[global] Instance pod_has_int32_member_key_decision sts pod :
+    Decision (pod_has_int32_member_key sts pod).
+Proof. unfold pod_has_int32_member_key. apply _. Defined.
+
+Definition missing_pod_keys sts (pods : list PodV.t) : list KKey.t :=
+  filter (λ key, key ∉ (PodV.key <$> pods)) (desired_pod_keys sts).
+
+Definition needed_pods sts pods : list PodV.t :=
+  filter (λ pod, pod_key_is_desired sts (PodV.key pod)) pods.
+
+Definition outdated_pods sts pods : list PodV.t :=
+  filter (λ pod, ¬ pod_match sts pod) (needed_pods sts pods).
+
+Definition bad_name_pods sts pods : list PodV.t :=
+  filter (λ pod, ¬ pod_has_int32_member_key sts pod) pods.
+
+Definition condemned_pods sts pods : list PodV.t :=
+  filter (λ pod,
+    pod_has_int32_member_key sts pod ∧
+    ¬ pod_key_is_desired sts (PodV.key pod)) pods.
+
+Definition pod_distance sts pods : nat :=
+  length (missing_pod_keys sts pods) +
+  2 * length (filter is_pod_alive (outdated_pods sts pods)) +
+  length (filter is_pod_alive (condemned_pods sts pods)) +
+  length (bad_name_pods sts pods).
+
+Definition missing_pvc_keys sts (pvcs : list PersistentVolumeClaimV.t) :
+    list KKey.t :=
+  filter (λ key, key ∉ (PersistentVolumeClaimV.key <$> pvcs))
+    (desired_pvc_keys sts).
+
+Definition pvc_distance sts pvcs : nat :=
+  length (missing_pvc_keys sts pvcs).
+
+Definition match_distance sts pods pvcs : nat :=
+  pod_distance sts pods + pvc_distance sts pvcs.
+
+Definition pods_match sts pods : Prop :=
+  PodV.key <$> pods ≡ₚ desired_pod_keys sts ∧
+  Forall is_pod_alive pods ∧
+  Forall (pod_match sts) pods.
+
+Definition pvcs_match sts (pvcs : list PersistentVolumeClaimV.t) : Prop :=
+  ∀ key, key ∈ desired_pvc_keys sts →
+    key ∈ (PersistentVolumeClaimV.key <$> pvcs).
+
+Definition current_state_matches sts pods pvcs : Prop :=
+  pods_match sts pods ∧ pvcs_match sts pvcs.
+
+Definition pod_meta_except_resource_version_changed
+    (pods pods' : list PodV.t) : Prop :=
+  ∃ pod pod',
+    pod ∈ pods ∧
+    pod' ∈ pods' ∧
+    PodV.key pod = PodV.key pod' ∧
+    ObjectMetaV.without_resource_version pod.(PodV.ObjectMeta') ≠
+      ObjectMetaV.without_resource_version pod'.(PodV.ObjectMeta').
+
+Definition pod_spec_changed (pods pods' : list PodV.t) : Prop :=
+  ∃ pod pod',
+    pod ∈ pods ∧
+    pod' ∈ pods' ∧
+    PodV.key pod = PodV.key pod' ∧
+    pod.(PodV.Spec') ≠ pod'.(PodV.Spec').
+
+Definition pods_progress_observed (pods pods' : list PodV.t) : Prop :=
+  list_to_set (C:=gset KKey.t) (PodV.key <$> pods) ≠
+    list_to_set (C:=gset KKey.t) (PodV.key <$> pods') ∨
+  pod_meta_except_resource_version_changed pods pods' ∨
+  pod_spec_changed pods pods'.
+
+Definition input_requirement (sts : StatefulSetV.t) : Prop :=
+  (* Generated Pod names are also hostnames and label values, so they must
+     remain within the DNS-1123 label limit after adding the ordinal. *)
+  (∀ ordinal,
+    (ordinal < statefulset_replicas sts)%nat →
+    valid_dns1123_label
+      (desired_pod_name
+        sts.(StatefulSetV.ObjectMeta').(ObjectMetaV.Name') ordinal)) ∧
+  (* StatefulSet admission does not validate Pod-template finalizers, although
+     Pod create validates the finalizers copied by the controller. *)
+  valid_finalizers
+    ((sts.(StatefulSetV.Spec').(StatefulSetSpecV.Template')).(
+      PodTemplateSpecV.ObjectMeta').(ObjectMetaV.Finalizers')) ∧
+  (* StatefulSet admission validates claim-template specs but not all metadata
+     copied to the PVC submitted by the controller. *)
+  Forall
+    (λ claim_template,
+      ∀ ordinal,
+        (ordinal < statefulset_replicas sts)%nat →
+        PersistentVolumeClaimV.valid_named_create
+          sts.(StatefulSetV.ObjectMeta').(ObjectMetaV.Namespace')
+          (new_persistent_volume_claim sts claim_template ordinal))
+    sts.(StatefulSetV.Spec').(StatefulSetSpecV.VolumeClaimTemplates').
+
+Section specs.
+Context `{hG: !heapGS Σ} `{!ffi_semantics _ _}.
+Context {sem : go.Semantics}
+  {package_sem : code.controllers.statefulset.statefulset.Assumptions}.
+Collection W := sem + package_sem.
+#[local] Instance base_common_sem : common.Assumptions | 100 :=
+  code.controllers.statefulset.statefulset.import_common_Assumption.
+#[local] Instance controller_sem : controller.Assumptions :=
+  code.controllers.statefulset.statefulset.import_controller_Assumption.
+#[local] Instance runtime_sem :
+    code.k8s_io.apimachinery.pkg.runtime.runtime.Assumptions :=
+  controller.import_runtime_Assumption.
+#[local] Instance runtime_object_underlying_eq :
+    runtime.Object ≤u runtime.Objectⁱᵐᵖˡ.
+Proof using package_sem. apply _. Qed.
+#[local] Instance meta_object_underlying_eq :
+    meta_v1.Object ≤u meta_v1.Objectⁱᵐᵖˡ.
+Proof using package_sem. apply _. Qed.
+#[local] Instance base_apimodel_sem : apimodel.Assumptions | 100 :=
+  common.import_apimodel_Assumption.
+#[local] Instance object_meta_v1_sem :
+    code.k8s_io.apimachinery.pkg.apis.meta.v1.v1.Assumptions :=
+  apimodel.import_apis_meta_v1_Assumption.
+#[local] Instance object_apps_v1_sem :
+    code.k8s_io.api.apps.v1.v1.Assumptions :=
+  apimodel.import_api_apps_v1_Assumption.
+#[local] Instance object_core_v1_sem :
+    code.k8s_io.api.core.v1.v1.Assumptions :=
+  code.k8s_io.api.apps.v1.v1.import_core_v1_Assumption.
+#[local] Instance apimodel_sem : apimodel.Assumptions | 0.
+Proof using package_sem.
+  constructor; try exact object_core_v1_sem; try apply _.
+Defined.
+#[local] Instance common_sem : common.Assumptions | 0.
+Proof using package_sem.
+  constructor; try exact apimodel_sem; try apply _.
+Defined.
+Context `{!kubernetesModelG Σ}.
+Local Set Default Proof Using "All".
+
+Definition syncStatefulSet_progress_spec γ l namespace name sts dq pods pvcs :
+    iProp Σ :=
+  {{{ is_pkg_init code.controllers.statefulset.pkg_id.statefulset ∗
+      "#Hisk" ∷ is_kubernetes γ l ∗
+      "#Hglobal_l" ∷ (global_addr apimodel.ModelState) ↦□ l ∗
+      "Hown_sts_meta_frag" ∷ own_meta_frag γ (StatefulSetV.key sts) sts.(StatefulSetV.ObjectMeta').(ObjectMetaV.UID') dq sts.(StatefulSetV.ObjectMeta') ∗
+      "Hown_sts_spec_frag" ∷ own_spec_frag γ (StatefulSetV.key sts) sts.(StatefulSetV.ObjectMeta').(ObjectMetaV.UID') dq (ObjectSpecV.StatefulSetSpec sts.(StatefulSetV.Spec')) ∗
+      "Hown_pod_frags" ∷ ([∗ list] pod ∈ pods,
+        own_meta_frag γ (PodV.key pod) pod.(PodV.ObjectMeta').(ObjectMetaV.UID') 1 pod.(PodV.ObjectMeta') ∗
+        own_spec_frag γ (PodV.key pod) pod.(PodV.ObjectMeta').(ObjectMetaV.UID') 1 (ObjectSpecV.PodSpec pod.(PodV.Spec'))) ∗
+      "Hown_pvc_frags" ∷ ([∗ list] pvc ∈ pvcs,
+        own_meta_frag γ (PersistentVolumeClaimV.key pvc) pvc.(PersistentVolumeClaimV.ObjectMeta').(ObjectMetaV.UID') 1 pvc.(PersistentVolumeClaimV.ObjectMeta')) ∗
+      "Hown_children_frag" ∷ own_children_frag γ (StatefulSetV.key sts) sts.(StatefulSetV.ObjectMeta').(ObjectMetaV.UID') 1 (list_to_set (PodV.key <$> pods)) ∗
+      "Hown_reserved_missing_pod_keys" ∷ ([∗ list] key ∈ missing_pod_keys sts pods, own_reserved_frag γ key) ∗
+      "Hown_reserved_missing_pvc_keys" ∷ ([∗ list] key ∈ missing_pvc_keys sts pvcs, own_reserved_frag γ key) ∗
+      "%Hpending_pods_empty" ∷ ⌜ filter (pending_pod sts) pods = [] ⌝ ∗
+      "%Hinput_requirement" ∷ ⌜ input_requirement sts ⌝ ∗
+      "%Hnamespace_eq" ∷ ⌜ namespace = sts.(StatefulSetV.ObjectMeta').(ObjectMetaV.Namespace') ⌝ ∗
+      "%Hname_eq" ∷ ⌜ name = sts.(StatefulSetV.ObjectMeta').(ObjectMetaV.Name') ⌝ ∗
+      "%Hdeletion_timestamp_eq" ∷ ⌜ sts.(StatefulSetV.ObjectMeta').(ObjectMetaV.DeletionTimestamp') = None ⌝
+  }}}
+    @! statefulset.syncStatefulSet #namespace #name
+  {{{ (pods' : list PodV.t) (pvcs' : list PersistentVolumeClaimV.t)
+      (err : interface.t), RET #err;
+      ⌜ current_state_matches sts pods' pvcs' ∨
+        pods_progress_observed pods pods' ∧
+          match_distance sts pods' pvcs' < match_distance sts pods pvcs ⌝ ∗
+      own_meta_frag γ (StatefulSetV.key sts) sts.(StatefulSetV.ObjectMeta').(ObjectMetaV.UID') dq sts.(StatefulSetV.ObjectMeta') ∗
+      own_spec_frag γ (StatefulSetV.key sts) sts.(StatefulSetV.ObjectMeta').(ObjectMetaV.UID') dq (ObjectSpecV.StatefulSetSpec sts.(StatefulSetV.Spec')) ∗
+      ([∗ list] pod ∈ pods',
+        own_meta_frag γ (PodV.key pod) pod.(PodV.ObjectMeta').(ObjectMetaV.UID') 1 pod.(PodV.ObjectMeta') ∗
+        own_spec_frag γ (PodV.key pod) pod.(PodV.ObjectMeta').(ObjectMetaV.UID') 1 (ObjectSpecV.PodSpec pod.(PodV.Spec'))) ∗
+      ([∗ list] pvc ∈ pvcs',
+        own_meta_frag γ (PersistentVolumeClaimV.key pvc) pvc.(PersistentVolumeClaimV.ObjectMeta').(ObjectMetaV.UID') 1 pvc.(PersistentVolumeClaimV.ObjectMeta')) ∗
+      own_children_frag γ (StatefulSetV.key sts) sts.(StatefulSetV.ObjectMeta').(ObjectMetaV.UID') 1 (list_to_set (PodV.key <$> pods'))
+  }}}.
+
+Definition syncStatefulSet_stability_spec γ l namespace name sts dq pods pvcs :
+    iProp Σ :=
+  {{{ is_pkg_init code.controllers.statefulset.pkg_id.statefulset ∗
+      "#Hisk" ∷ is_kubernetes γ l ∗
+      "#Hglobal_l" ∷ (global_addr apimodel.ModelState) ↦□ l ∗
+      "Hown_sts_meta_frag" ∷ own_meta_frag γ (StatefulSetV.key sts) sts.(StatefulSetV.ObjectMeta').(ObjectMetaV.UID') dq sts.(StatefulSetV.ObjectMeta') ∗
+      "Hown_sts_spec_frag" ∷ own_spec_frag γ (StatefulSetV.key sts) sts.(StatefulSetV.ObjectMeta').(ObjectMetaV.UID') dq (ObjectSpecV.StatefulSetSpec sts.(StatefulSetV.Spec')) ∗
+      "Hown_pod_frags" ∷ ([∗ list] pod ∈ pods,
+        own_meta_frag γ (PodV.key pod) pod.(PodV.ObjectMeta').(ObjectMetaV.UID') dq pod.(PodV.ObjectMeta') ∗
+        own_spec_frag γ (PodV.key pod) pod.(PodV.ObjectMeta').(ObjectMetaV.UID') dq (ObjectSpecV.PodSpec pod.(PodV.Spec'))) ∗
+      "Hown_pvc_frags" ∷ ([∗ list] pvc ∈ pvcs,
+        own_meta_frag γ (PersistentVolumeClaimV.key pvc) pvc.(PersistentVolumeClaimV.ObjectMeta').(ObjectMetaV.UID') dq pvc.(PersistentVolumeClaimV.ObjectMeta')) ∗
+      "Hown_children_frag" ∷ own_children_frag γ (StatefulSetV.key sts) sts.(StatefulSetV.ObjectMeta').(ObjectMetaV.UID') dq (list_to_set (PodV.key <$> pods)) ∗
+      "%Hnamespace_eq" ∷ ⌜ namespace = sts.(StatefulSetV.ObjectMeta').(ObjectMetaV.Namespace') ⌝ ∗
+      "%Hname_eq" ∷ ⌜ name = sts.(StatefulSetV.ObjectMeta').(ObjectMetaV.Name') ⌝ ∗
+      "%Hdeletion_timestamp_eq" ∷ ⌜ sts.(StatefulSetV.ObjectMeta').(ObjectMetaV.DeletionTimestamp') = None ⌝ ∗
+      "%Hmatch" ∷ ⌜ current_state_matches sts pods pvcs ⌝
+  }}}
+    @! statefulset.syncStatefulSet #namespace #name
+  {{{ (err : interface.t), RET #err;
+      own_meta_frag γ (StatefulSetV.key sts) sts.(StatefulSetV.ObjectMeta').(ObjectMetaV.UID') dq sts.(StatefulSetV.ObjectMeta') ∗
+      own_spec_frag γ (StatefulSetV.key sts) sts.(StatefulSetV.ObjectMeta').(ObjectMetaV.UID') dq (ObjectSpecV.StatefulSetSpec sts.(StatefulSetV.Spec')) ∗
+      ([∗ list] pod ∈ pods,
+        own_meta_frag γ (PodV.key pod) pod.(PodV.ObjectMeta').(ObjectMetaV.UID') dq pod.(PodV.ObjectMeta') ∗
+        own_spec_frag γ (PodV.key pod) pod.(PodV.ObjectMeta').(ObjectMetaV.UID') dq (ObjectSpecV.PodSpec pod.(PodV.Spec'))) ∗
+      ([∗ list] pvc ∈ pvcs,
+        own_meta_frag γ (PersistentVolumeClaimV.key pvc) pvc.(PersistentVolumeClaimV.ObjectMeta').(ObjectMetaV.UID') dq pvc.(PersistentVolumeClaimV.ObjectMeta')) ∗
+      own_children_frag γ (StatefulSetV.key sts) sts.(StatefulSetV.ObjectMeta').(ObjectMetaV.UID') dq (list_to_set (PodV.key <$> pods))
+  }}}.
+
+Definition syncStatefulSet_preservation_spec γ l namespace name sts dq
+    pending_dqs pods pvcs : iProp Σ :=
+  {{{ is_pkg_init code.controllers.statefulset.pkg_id.statefulset ∗
+      "#Hisk" ∷ is_kubernetes γ l ∗
+      "#Hglobal_l" ∷ (global_addr apimodel.ModelState) ↦□ l ∗
+      "Hown_sts_meta_frag" ∷ own_meta_frag γ (StatefulSetV.key sts) sts.(StatefulSetV.ObjectMeta').(ObjectMetaV.UID') dq sts.(StatefulSetV.ObjectMeta') ∗
+      "Hown_sts_spec_frag" ∷ own_spec_frag γ (StatefulSetV.key sts) sts.(StatefulSetV.ObjectMeta').(ObjectMetaV.UID') dq (ObjectSpecV.StatefulSetSpec sts.(StatefulSetV.Spec')) ∗
+      "Hown_terminating_pod_frags" ∷
+        ([∗ list] pod;pending_dq ∈ filter (pending_pod sts) pods;pending_dqs,
+          own_meta_frag γ (PodV.key pod) pod.(PodV.ObjectMeta').(ObjectMetaV.UID') pending_dq pod.(PodV.ObjectMeta') ∗
+          own_spec_frag γ (PodV.key pod) pod.(PodV.ObjectMeta').(ObjectMetaV.UID') pending_dq (ObjectSpecV.PodSpec pod.(PodV.Spec'))) ∗
+      "Hown_other_pod_frags" ∷
+        ([∗ list] pod ∈ filter (λ pod, not (pending_pod sts pod)) pods,
+          own_meta_frag γ (PodV.key pod) pod.(PodV.ObjectMeta').(ObjectMetaV.UID') 1 pod.(PodV.ObjectMeta') ∗
+          own_spec_frag γ (PodV.key pod) pod.(PodV.ObjectMeta').(ObjectMetaV.UID') 1 (ObjectSpecV.PodSpec pod.(PodV.Spec'))) ∗
+      "Hown_pvc_frags" ∷ ([∗ list] pvc ∈ pvcs,
+        own_meta_frag γ (PersistentVolumeClaimV.key pvc) pvc.(PersistentVolumeClaimV.ObjectMeta').(ObjectMetaV.UID') 1 pvc.(PersistentVolumeClaimV.ObjectMeta')) ∗
+      "Hown_children_frag" ∷ own_children_frag γ (StatefulSetV.key sts) sts.(StatefulSetV.ObjectMeta').(ObjectMetaV.UID') 1 (list_to_set (PodV.key <$> pods)) ∗
+      "Hown_reserved_missing_pod_keys" ∷ ([∗ list] key ∈ missing_pod_keys sts pods, own_reserved_frag γ key) ∗
+      "Hown_reserved_missing_pvc_keys" ∷ ([∗ list] key ∈ missing_pvc_keys sts pvcs, own_reserved_frag γ key) ∗
+      "%Hpods_nodup" ∷ ⌜ NoDup (PodV.key <$> pods) ⌝ ∗
+      "%Hpending_nonempty" ∷ ⌜ filter (pending_pod sts) pods ≠ [] ⌝ ∗
+      "%Hinput_requirement" ∷ ⌜ input_requirement sts ⌝ ∗
+      "%Hnamespace_eq" ∷ ⌜ namespace = sts.(StatefulSetV.ObjectMeta').(ObjectMetaV.Namespace') ⌝ ∗
+      "%Hname_eq" ∷ ⌜ name = sts.(StatefulSetV.ObjectMeta').(ObjectMetaV.Name') ⌝ ∗
+      "%Hdeletion_timestamp_eq" ∷ ⌜ sts.(StatefulSetV.ObjectMeta').(ObjectMetaV.DeletionTimestamp') = None ⌝
+  }}}
+    @! statefulset.syncStatefulSet #namespace #name
+  {{{ (pods' : list PodV.t) (pvcs' : list PersistentVolumeClaimV.t)
+      (err : interface.t), RET #err;
+      ⌜ match_distance sts pods' pvcs' ≤ match_distance sts pods pvcs ⌝ ∗
+      ⌜ filter (pending_pod sts) pods ⊆ filter (pending_pod sts) pods' ⌝ ∗
+      own_meta_frag γ (StatefulSetV.key sts) sts.(StatefulSetV.ObjectMeta').(ObjectMetaV.UID') dq sts.(StatefulSetV.ObjectMeta') ∗
+      own_spec_frag γ (StatefulSetV.key sts) sts.(StatefulSetV.ObjectMeta').(ObjectMetaV.UID') dq (ObjectSpecV.StatefulSetSpec sts.(StatefulSetV.Spec')) ∗
+      ([∗ list] pod;pending_dq ∈ filter (pending_pod sts) pods;pending_dqs,
+        own_meta_frag γ (PodV.key pod) pod.(PodV.ObjectMeta').(ObjectMetaV.UID') pending_dq pod.(PodV.ObjectMeta') ∗
+        own_spec_frag γ (PodV.key pod) pod.(PodV.ObjectMeta').(ObjectMetaV.UID') pending_dq (ObjectSpecV.PodSpec pod.(PodV.Spec'))) ∗
+      ([∗ list] pod ∈ filter (λ pod,
+          PodV.key pod ∉ PodV.key <$> filter (pending_pod sts) pods) pods',
+        own_meta_frag γ (PodV.key pod) pod.(PodV.ObjectMeta').(ObjectMetaV.UID') 1 pod.(PodV.ObjectMeta') ∗
+        own_spec_frag γ (PodV.key pod) pod.(PodV.ObjectMeta').(ObjectMetaV.UID') 1 (ObjectSpecV.PodSpec pod.(PodV.Spec'))) ∗
+      ([∗ list] pvc ∈ pvcs',
+        own_meta_frag γ (PersistentVolumeClaimV.key pvc) pvc.(PersistentVolumeClaimV.ObjectMeta').(ObjectMetaV.UID') 1 pvc.(PersistentVolumeClaimV.ObjectMeta')) ∗
+      own_children_frag γ (StatefulSetV.key sts) sts.(StatefulSetV.ObjectMeta').(ObjectMetaV.UID') 1 (list_to_set (PodV.key <$> pods'))
+  }}}.
+
+End specs.
