src/proof/controllers/statefulset/update_pod.v
@@ -1,3 +1,4 @@
+From New.proof.controllers.statefulset Require Import top_level.
 From New.proof.controllers.statefulset Require Export pod_identity.
 From New.proof.k8s_io.api.core Require Export v1.
 From New.proof.kubernetes_model.tx Require Export update.
